Latest changes

apa.v
@@ -3,28 +3,56 @@ Require Import Coq.Lists.List.
 Require Import job.
 Require Import schedule.
 Require Import helper.
+Require Import identmp.
 
-Definition affinity := job -> schedule -> list nat.
+Definition affinity := job -> list nat.
 
-Record apa_ident_mp (num_cpus: nat) (sched: schedule) (alpha: affinity) : Prop :=
-  { apa_ident_is_ident: ident_mp num_cpus sched;
-    restricted_affinities:
-        forall (t: time),
-            (forall (l: list (option job)) (j: job) (cpu: nat),
+Record apa_ident_mp (num_cpus: nat) (sched: schedule) (alpha: affinity) (hp: higher_priority) : Prop :=
+  { apa_ident_mp_cpus_nonzero: num_cpus > 0;
+
+    (* Job is scheduled iff it is mapped to a processor*)
+    apa_ident_mp_mapping: forall (t: time),
+                          (length (cpumap sched t) = num_cpus /\
+                          (forall (j: job),
+                              List.In (Some j) (cpumap sched t) <-> sched j t = 1));
+    apa_ident_mp_sched_unit: forall (j: job) (t: time), sched j t <= 1;
+
+    (* If some job is scheduled, then its affinity should allow it. *)
+    apa_ident_mp_restricted_affinities:
+        forall (t: time) (j: job) (cpu: nat),
                 sched j t = 1 ->
                 cpu < num_cpus ->
-                (nth cpu l (Some j) = Some j) ->
-                List.In cpu (alpha j sched))
+                (nth cpu (cpumap sched t) (Some j) = Some j) ->
+                List.In cpu (alpha j);
+
+    (* (Weak) APA scheduling invariant *)
+    apa_ident_mp_invariant:
+        forall (jlow: job) (t: time),
+            backlogged jlow sched t <->
+                (forall (cpu: nat),
+                cpu < num_cpus /\
+                List.In cpu (alpha jlow) ->
+                    (exists (jhigh: job),
+                        (nth cpu (cpumap sched t) (Some jhigh) = Some jhigh)))
   }.
 
 Lemma exists_apa_platform_that_is_global :
-    forall (num_cpus: nat) (s: schedule),
-        ident_mp num_cpus s ->
+    forall (num_cpus: nat) (s: schedule) (hp: higher_priority),
+        ident_mp num_cpus s hp ->
         exists (s': schedule) (alpha: affinity),
-            apa_ident_mp num_cpus s alpha
+            apa_ident_mp num_cpus s alpha hp
             /\ (forall (j: job) (t: time), service s j t = service s' j t).
-Proof. intros. exists s. exists (fun (j : job) (s: schedule) => (seq 0 num_cpus)).
-       split. split. apply H.
+Proof. intros. inversion H. exists s. exists (fun (j : job) => (seq 0 num_cpus)).
+       split. split.
+       apply ident_mp_cpus_nonzero.
+       apply ident_mp_mapping.
+       apply ident_mp_sched_unit.
        intros. apply nat_seq_nth_In. apply H1.
-       trivial.
+       intros. assert (H1 := ident_mp_invariant jlow t).
+       inversion H1. split.
+       intros. assert (H5 := H0 H3 cpu). inversion H4.
+       apply H5 in H6. trivial.
+       intros. apply H2. intros.
+       assert (H5 := H3 cpu). assert (H6 := nat_seq_nth_In num_cpus cpu H4).
+       assert (H7 := H5 (conj H4 H6)). trivial. trivial.
 Qed.
