identmp.v
@@ -3,12 +3,24 @@ Require Import Coq.Lists.List.
 Require Import job.
 Require Import schedule.
 
-Record ident_mp (num_cpus: nat) (sched: schedule) : Prop :=
+Axiom cpumap : schedule -> time -> list (option job).
+
+Record ident_mp (num_cpus: nat) (sched: schedule) (hp: higher_priority) : Prop :=
   { ident_mp_cpus_nonzero: num_cpus > 0;
+
+    (* Job is scheduled iff it is mapped to a processor*)
     ident_mp_mapping: forall (t: time),
-                          (exists !(l: list (option job)),
-                              length l = num_cpus /\
-                              (forall (j: job),
-                                  List.In (Some j) l <-> sched j t = 1));
-    ident_mp_sched_unit: forall (j: job) (t: time), sched j t <= 1
+                          (length (cpumap sched t) = num_cpus /\
+                          (forall (j: job),
+                              List.In (Some j) (cpumap sched t) <-> sched j t = 1));
+    ident_mp_sched_unit: forall (j: job) (t: time), sched j t <= 1;
+
+    (* Global scheduling invariant *)
+    ident_mp_invariant:
+        forall (jlow: job) (t: time),
+            backlogged jlow sched t <->
+                (forall (cpu: nat),
+                cpu < num_cpus ->
+                    (exists (jhigh: job),
+                        (nth cpu (cpumap sched t) (Some jhigh) = Some jhigh)))
   }.
