liulayland.v
@@ -3,8 +3,24 @@ Require Import Coq.Lists.List.
 Require Import job.
 Require Import schedule.
 Require Import identmp.
+Require Import priority.
 
 Section LiuLayland.
 Variable sched: schedule.
-Axiom uniprocessor : ident_mp 1 sched.
+Variable hp: higher_priority.
+Axiom RM_priority : fixed_priority hp RM.
+Axiom uniprocessor : ident_mp 1 sched hp.
+
+Lemma uni_simpler_invariant : forall (jlow : job) (t : time),
+                backlogged jlow sched t <-> exists ! jhigh : job, sched jhigh t = 1.
+Proof.
+  intros.
+  assert (H1 := uniprocessor).
+  split.
+  intros. unfold backlogged in H. inversion H.
+  inversion H1.
+  assert (H3 := ident_mp_invariant jlow t).
+  inversion H3.
+
+
 End LiuLayland.
